[statelib examples] wip on pncounter proof.

aneris/examples/crdt/statelib/examples/pncounter/pncounter_proof.v
@@ -74,13 +74,8 @@ Section pn_cpt_proof.
 
 End pn_cpt_proof.
 
-Section pncounter_proof.
-
-  Context `{!anerisG M Σ, !CRDT_Params, pnRes : !StLib_Res (prodOp gctr_op gctr_op)}.
-
-  Notation pnOp := (prodOp gctr_op gctr_op).
-  Notation pnSt := (prodSt gctr_st gctr_st).
-  Notation pnParams := (prod_params gctr_op gctr_st gctr_op gctr_st).
+Section Util.
+  Context `{!anerisG M Σ}.
 
   Lemma wp_list_int_sum (l : list nat) lv ip :
     {{{ ⌜is_list l lv⌝ }}}
@@ -105,9 +100,207 @@ Section pncounter_proof.
       by iApply "HΦ".
   Qed.
 
-  Definition pn_upd_spec := (@update_spec pnOp pnSt _ _ _ _ _ _ (prod_crdt_coh_params _ _ _ _) pnRes).
-  Definition pn_get_state_spec := (@get_state_spec pnOp pnSt _ _ _ _ _ _ _ (prod_crdt_coh_params _ _ _ _) pnRes).
+End Util.
 
+Section pncounter_denot.
+
+  Context `{!anerisG M Σ}.
+  Context `{!CRDT_Params}.
+
+  Inductive CtrOp :=
+  | Add (z : Z) : CtrOp.
+
+  Definition ctr_payload (op : CtrOp) : Z :=
+    match op with
+    | Add z => z
+    end.
+
+  Global Instance ctr_op_eqdecision : EqDecision CtrOp.
+  Proof. solve_decision. Qed.
+
+  Global Instance ctr_op_countable : Countable CtrOp.
+  Proof.
+    refine {|
+      encode op := match op with Add z => encode z end;
+      decode n := Add <$> @decode Z _ _ n;
+    |}.
+    intros []. rewrite decode_encode /=. done.
+  Qed.
+
+  Definition CtrSt := Z.
+  (* Context `{!Log_Time}. *)
+
+  (* The value of a counter is just the sum of the operations' payloads. *)
+  Fixpoint ctr_value (s : list (Event CtrOp)) : Z :=
+    match s with
+    | [] => 0%Z
+    | ev :: xs => (ctr_payload ev.(EV_Op) + ctr_value xs)%Z
+    end.
+
+  Definition ctr_denot (s : gset (Event CtrOp)) (st : CtrSt) : Prop :=
+    st = ctr_value (elements s).
+
+  Global Instance ctr_denot_fun : Rel2__Fun ctr_denot.
+  Proof.
+    constructor; unfold ctr_denot; intros; subst; done.
+  Qed.
+
+  Global Instance ctr_denot_instance : CrdtDenot CtrOp CtrSt := {
+    crdt_denot := ctr_denot;
+  }.
+
+  Lemma ctr_value_singleton ev :
+    ctr_value [ev] = ctr_payload (ev.(EV_Op)).
+  Proof.
+    unfold ctr_value. lia.
+  Qed.
+
+  Lemma ctr_value_cons ev l :
+    ctr_value (ev :: l) = (ctr_payload ev.(EV_Op) + ctr_value l)%Z.
+  Proof.
+    simpl. auto.
+  Qed.
+
+  Lemma ctr_value_app (l l' : list (Event CtrOp)) :
+    ctr_value (l ++ l') = (ctr_value l + ctr_value l')%Z.
+  Proof.
+    generalize dependent l'.
+    induction l as [ | h t Ht]; intros l'; [done |].
+    rewrite -app_comm_cons.
+    do 2 rewrite ctr_value_cons.
+    rewrite (Ht l'). lia.
+  Qed.
+
+  Lemma ctr_value_perm (l l' : list (Event CtrOp)) :
+    Permutation l l' -> ctr_value l = ctr_value l'.
+  Proof.
+    generalize dependent l'.
+    induction l as [ | h t Ht]; intros l' Hperm.
+    - apply Permutation_nil in Hperm; subst; reflexivity.
+    - rewrite ctr_value_cons.
+      apply Permutation_sym in Hperm.
+      pose proof Hperm as Hperm'.
+      apply Permutation_vs_cons_inv in Hperm as [l1 [l2 ->]].
+      apply Permutation_sym, Permutation_cons_app_inv, Ht in Hperm'.
+      rewrite Hperm'.
+      do 2 rewrite ctr_value_app.
+      rewrite ctr_value_cons.
+      lia.
+  Qed.
+
+End pncounter_denot.
+
+Section pncounter_coh.
+
+  Context `{!anerisG M Σ}.
+  Context `{!CRDT_Params}.
+
+  Definition Ctr_Op_Coh := λ (op : CtrOp) v, match op with Add z => v = #z end.
+
+  Lemma Ctr_Op_Coh_Inj (o1 o2 : CtrOp) (v : val) :
+    Ctr_Op_Coh o1 v → Ctr_Op_Coh o2 v → o1 = o2.
+  Proof. destruct o1; destruct o2; simpl; intros ? ?; simplify_eq; done. Qed.
+
+  Lemma Ctr_Op_Coh_Ser (op : CtrOp) (v : val) :
+    Ctr_Op_Coh op v → Serializable int_serialization v.
+  Proof.
+    destruct op; rewrite /Ctr_Op_Coh; intros ?; simplify_eq; apply _.
+  Qed.
+
+  Definition Ctr_St_Coh := λ (st : CtrSt) v, v = #st.
+
+
+  Lemma Ctr_St_Coh_Inj st1 st2 v :
+    Ctr_St_Coh st1 v → Ctr_St_Coh st2 v → st1 = st2.
+  Proof. rewrite /Ctr_St_Coh. intros. by simplify_eq. Qed.
+
+  Lemma Ctr_St_Coh_Ser (st : CtrSt) (v : val) :
+    Ctr_St_Coh st v → Serializable int_serialization v.
+  Proof. rewrite /Ctr_St_Coh; intros ?; simplify_eq; apply _. Qed.
+
+
+  Global Instance Ctr_Coh_Params : @StLib_Coh_Params CtrOp CtrSt :=
+  {|
+    StLib_StSerialization := int_serialization;
+    StLib_Op_Coh := Ctr_Op_Coh;
+    StLib_Op_Coh_Inj := Ctr_Op_Coh_Inj;
+    StLib_St_Coh := Ctr_St_Coh;
+    StLib_St_Coh_Inj := Ctr_St_Coh_Inj;
+    StLib_StCoh_Ser := Ctr_St_Coh_Ser
+  |}.
+
+End pncounter_coh.
+
+Section pn_event_mapping.
+  Context `{!anerisG M Σ}.
+  Context `{!CRDT_Params}.
+
+  Notation pn_prod_Op := (prodOp gctr_op gctr_op).
+
+  Definition event_prod_of_Z (ev : Event CtrOp) : Event pn_prod_Op :=
+    let z := ctr_payload ev.(EV_Op) in
+    let op := if bool_decide (Z.le 0 z) then (Z.to_nat z, 0) else (0, Z.to_nat (-z)) in
+   {| EV_Op := op ;  EV_Orig := ev.(EV_Orig);  EV_Time := ev.(EV_Time) |}.
+
+  Definition event_set_prod_of_Z (s : event_set CtrOp) : event_set pn_prod_Op :=
+    gset_map (λ ev, event_prod_of_Z ev) s.
+
+  Definition event_Z_of_prod (ev : Event pn_prod_Op) : Event CtrOp :=
+    let (p,n) := ev.(EV_Op) in
+    {| EV_Op := Add (p-n);  EV_Orig := ev.(EV_Orig);  EV_Time := ev.(EV_Time) |}.
+
+  Definition event_set_Z_of_prod (s : event_set pn_prod_Op) : event_set CtrOp :=
+    gset_map (λ ev, event_Z_of_prod ev) s.
+
+End pn_event_mapping.
+
+Section pn_Res_mapping.
+  Context `{!anerisG M Σ}.
+  Context `{!CRDT_Params}.
+  Context `{pn_prod_Res : !StLib_Res (prodOp gctr_op gctr_op)}.
+
+  Global Program Instance pn_Res : StLib_Res CtrOp :=
+    {|
+      StLib_InitToken := pn_prod_Res.(StLib_InitToken);
+      StLib_SocketProto := pn_prod_Res.(StLib_SocketProto);
+    |}.
+  Next Obligation.
+  Admitted.
+
+End pn_Res_mapping.
+
+Section pn_prod_specs_def.
+  Context `{!anerisG M Σ}.
+  Context `{!CRDT_Params}.
+  Context `{pn_prod_Res : !StLib_Res (prodOp gctr_op gctr_op)}.
+
+  Notation pn_prod_Op := (prodOp gctr_op gctr_op).
+  Notation pn_prod_St := (prodSt gctr_st gctr_st).
+  Notation pn_prod_Params := (prod_params gctr_op gctr_st gctr_op gctr_st).
+
+  Definition pn_prod_upd_spec := (@update_spec pn_prod_Op pn_prod_St _ _ _ _ _ _ (prod_crdt_coh_params _ _ _ _) pn_prod_Res).
+  Definition pn_prod_get_state_spec := (@get_state_spec pn_prod_Op pn_prod_St _ _ _ _ _ _ _ (prod_crdt_coh_params _ _ _ _) pn_prod_Res).
+  Definition pn_prod_init_crdt_spec :=
+    @init_spec_for_specific_crdt pn_prod_Op pn_prod_St _ _ _ _ _ _ _ (prod_crdt_coh_params _ _ _ _) pn_prod_Res.
+
+End pn_prod_specs_def.
+
+Section pn_specs_def.
+  Context `{!anerisG M Σ}.
+  Context `{!CRDT_Params}.
+  Context `{pn_Res : !StLib_Res CtrOp}.
+
+  Definition pn_get_state_spec := (@get_state_spec CtrOp CtrSt _ _ _ _ _ _ _ Ctr_Coh_Params pn_Res).
+  Definition pn_upd_spec := @update_spec CtrOp CtrSt _ _ _ _ _ _ Ctr_Coh_Params pn_Res.
+  Definition pn_init_crdt_spec :=
+    @init_spec_for_specific_crdt CtrOp CtrSt _ _ _ _ _ _ _ Ctr_Coh_Params pn_Res.
+
+End pn_specs_def.
+
+Section pncounter_proof.
+  Context `{!anerisG M Σ}.
+  Context `{!CRDT_Params}.
+  Context `{pn_prod_Res : !StLib_Res (prodOp gctr_op gctr_op)}.
 
   (* TODO: Prove: *)
   (* Definition pncounter_update : val := *)
@@ -115,14 +308,9 @@ Section pncounter_proof.
   (*     (if: #0 ≤ "n" *)
   (*      then  "upd" ("n", #0) *)
   (*      else  "upd" (#0, (- "n"))). *)
-
-  (* NB: this is not what we want in the end. We want rather an
-     @update_spec with a logical state being Z. *)
-  Lemma pncounter_update_spec (upd_fn : val) (n : Z) repId addr:
-    pn_upd_spec upd_fn repId addr -∗
-    {{{ ⌜True⌝ }}}
-      pncounter_update upd_fn #n @[ip_of_address addr]
-    {{{ (n : nat),  RET #n; ⌜n = n⌝ }}}.
+  Lemma pncounter_update_spec (upd_fn : val) repId addr:
+    pn_prod_upd_spec upd_fn repId addr -∗
+    pn_upd_spec (λ:"n", pncounter_update upd_fn "n") repId addr.
   Proof. Admitted.
 
 
@@ -135,14 +323,9 @@ Section pncounter_proof.
   (*      let: "p" := list_int_sum "pl" in *)
   (*      let: "n" := list_int_sum "nl" in *)
   (*      "p" - "n". *)
-
- (* NB: this is not what we want in the end. We want rather an
-     @get_state_spec with a logical state being Z. *)
   Lemma pncounter_eval_spec (get_state_fn : val) repId addr:
-    pn_get_state_spec get_state_fn repId addr -∗
-    {{{ ⌜True⌝ }}}
-      pncounter_eval get_state_fn #() @[ip_of_address addr]
-    {{{ (n : nat),  RET #n; ⌜n = n⌝ }}}.
+    pn_prod_get_state_spec get_state_fn repId addr -∗
+    pn_get_state_spec (λ:<>, pncounter_update get_state_fn #()) repId addr.
   Proof. Admitted.
 
   (* TODO: Prove: *)
@@ -154,5 +337,9 @@ Section pncounter_proof.
   (*     let: "get" := pncounter_eval "get_st" in *)
   (*     let: "upd" := pncounter_update "upd_st" in *)
   (*     ("get", "upd"). *)
+  Lemma pncounter_init_crdt_spec :
+    pn_prod_init_crdt_spec pn_cpt_init -∗
+    pn_init_crdt_spec pncounter_init.
+  Proof. Admitted.
 
 End pncounter_proof.
