aneris/examples/crdt/statelib/examples/pncounter/pncounter_use_case.v
@@ -1,0 +1,491 @@
+From stdpp Require Import base gmap.
+From aneris.aneris_lang.lib Require Import list_proof.
+From iris.algebra Require Import excl.
+From iris.base_logic.lib Require Import invariants.
+From iris.proofmode Require Import tactics.
+From trillium.prelude Require Import finitary.
+From aneris.aneris_lang Require Import adequacy.
+From aneris.aneris_lang.program_logic Require Import aneris_adequacy.
+From aneris.aneris_lang.lib.serialization Require Import serialization_proof.
+From aneris.aneris_lang.lib Require Import inject.
+From aneris.aneris_lang Require Import aneris_lifting proofmode.
+From aneris.examples.crdt.spec Require Import crdt_base crdt_time crdt_events crdt_denot crdt_resources.
+From aneris.examples.crdt.statelib.user_model
+     Require Import semi_join_lattices model params.
+From aneris.examples.crdt.statelib Require Import statelib_code.
+From aneris.examples.crdt.statelib.time Require Import time.
+From aneris.examples.crdt.statelib.STS Require Import lst.
+From aneris.examples.crdt.statelib.proof
+     Require Import events spec.
+From aneris.examples.crdt.statelib.examples.gcounter
+     Require Import gcounter_proof.
+From aneris.examples.crdt.statelib.examples.prod_comb
+     Require Import prod_comb_proof.
+From aneris.examples.crdt.statelib.examples.pncounter
+     Require Import pncounter_code_wrapper pncounter_proof.
+
+Definition addresses := [SocketAddressInet "1.1.1.1" 100; SocketAddressInet "1.1.1.2" 100].
+Definition addresses_val : val := $ [SocketAddressInet "1.1.1.1" 100; SocketAddressInet "1.1.1.2" 100].
+
+
+Program Instance pnc_use_case_CRDT_Params : CRDT_Params :=
+  {| CRDT_Addresses := addresses;
+    CRDT_InvName := nroot .@ "gi_pnuc"|}.
+Next Obligation.
+Proof. repeat constructor; set_solver. Qed.
+
+Definition use_case_program1 : expr :=
+  let: "init_res" := pncounter_init addresses_val #0%nat in
+  let: "get" := Fst "init_res" in
+  let: "update" := Snd "init_res" in
+  "update" #1;;
+  let: "r" := "get" #() in
+  assert: ("r" = #1) || ("r" = #3).
+
+Definition use_case_program2 : expr :=
+  let: "init_res" := pncounter_init addresses_val #1%nat in
+  let: "get" := Fst "init_res" in
+  let: "update" := Snd "init_res" in
+  "update" #2;;
+  let: "r" := "get" #() in
+  assert: ("r" = #2) || ("r" = #3).
+
+Definition use_case_program : expr :=
+  Start "1.1.1.1" use_case_program1;;
+  Start "1.1.1.2" use_case_program2.
+
+(* TODO: move this more usefule version of the lemma to its approporate place. *)
+Lemma LocSnap_GlobSnap_Provenance' `{!anerisG Mdl Σ} `{!CRDT_Params} `{!Log_Time}
+    `{!EqDecision CRDT_Op} `{!Countable CRDT_Op} `{!crdt_resources.CRDT_Res_Mixin Mdl Σ CRDT_Op}
+    E i s1 s2 h:
+  ↑CRDT_InvName ⊆ E → GlobInv -∗ GlobSnap h -∗ LocSnap i s1 s2 ={E}=∗
+  ∃ h' : event_set CRDT_Op, GlobSnap h' ∗ ⌜s1 ∪ s2 ⊆ h'⌝ ∗ ⌜h ⊆ h'⌝.
+Proof.
+  iIntros (?) "#Hinv #HGsnap #HLsnap".
+  set (s := s1 ∪ s2).
+  assert (s ⊆ s1 ∪ s2) as Hs by set_solver.
+  clearbody s.
+  iInduction s as [|ev h'] "IH" using set_ind_L forall (s1 s2 Hs) "HLsnap".
+  - iModIntro. iExists _; iFrame "#"; iSplit; iPureIntro; set_solver.
+  - iMod ("IH" with "[] HLsnap") as (h'') "(HGsnap' & % & %)"; first by iPureIntro; set_solver.
+    iMod (LocSnap_GlobSnap_Provenance _ _ _ _ ev with "[//] HLsnap") as (h3) "[HGsnap3 %]";
+      [set_solver|set_solver|].
+    iModIntro.
+    iDestruct (GlobSnap_Union with "HGsnap' HGsnap3") as "HGsnap'".
+    iExists (h'' ∪ h3); iFrame.
+    iPureIntro; split; set_solver.
+Qed.
+
+Section use_case_proof.
+  Context `{!anerisG M Σ} `{!inG Σ (exclR unitO)}.
+  (* Context `{stparams0 : !StLib_Res (prodOp gctr_op gctr_op)}. *)
+  Context `{!StLib_Res CtrOp}.
+  Definition use_case_inv_name := nroot .@ "pnuc".
+
+  Definition use_case_inv `{!StLib_Res CtrOp} γ1 γ2 : iProp Σ :=
+    ∃ ges, GlobState ges ∗
+      (⌜ges = ∅⌝ ∨
+       (∃ ev, ⌜ges = {[ev]} ∧ EV_Op ev = Add 1 ∧ EV_Orig ev = 0%nat⌝ ∗ own γ1 (Excl ())) ∨
+       (∃ ev, ⌜ges = {[ev]} ∧ EV_Op ev = Add 2 ∧ EV_Orig ev = 1%nat⌝ ∗ own γ2 (Excl ())) ∨
+       (∃ ev1 ev2, ⌜ges = {[ev1; ev2]} ∧
+          EV_Op ev1 = Add 1 ∧ EV_Orig ev1 = 0%nat ∧
+          EV_Op ev2 = Add 2 ∧ EV_Orig ev2 = 1%nat⌝ ∗
+          own γ1 (Excl ()) ∗ own γ2 (Excl ()))).
+
+  Program Definition Ofin : fin (length addresses).
+  Proof. apply (@Fin.of_nat_lt 0 (length addresses)); simpl; lia.  Defined.
+
+  Lemma wp_use_case_program1  γ1 γ2 :
+    {{{ GlobInv ∗ StLib_InitToken Ofin ∗ pn_init_crdt_spec pncounter_init ∗
+        ([∗ list] i↦z ∈ CRDT_Addresses, z ⤇ StLib_SocketProto) ∗
+        SocketAddressInet "1.1.1.1" 100 ⤳ (∅, ∅) ∗ free_ports "1.1.1.1" {[100%positive]} ∗
+        inv use_case_inv_name (use_case_inv γ1 γ2) ∗ own γ1 (Excl ()) }}}
+      use_case_program1 @["1.1.1.1"]
+    {{{ RET #(); True }}}.
+  Proof.
+    iIntros (Φ)
+      "(#HGinv & Hcrdt_tk & Hinit & #Hprotos & Hsa & Hfp & #Hinv & Htok) HΦ".
+    rewrite /use_case_program1.
+    wp_apply ("Hinit" $! _ (SocketAddressInet "1.1.1.1" 100) addresses_val
+               with "[$Hsa $Hfp $Hcrdt_tk]").
+    { iFrame "#".
+      iSplit; first by iPureIntro; apply is_list_inject.
+      iPureIntro; set_solver. }
+    iIntros (get upd) "(Hls & #Hget & #Hupd)".
+    wp_pures.
+    wp_apply ("Hupd" $! _ (Add _)); [done|done|].
+    iInv use_case_inv_name as (ges) ">[HGs Hstate]" "Hclose".
+    iMod fupd_mask_subseteq as "Hmask"; [|iModIntro]; [solve_ndisj|].
+    iExists _, _, _; iFrame.
+    iNext.
+    iIntros (add_1_ev h' s1' s2').
+    rewrite !left_id_L.
+    iIntros "(%Hadd_1_val & %Hadd_1_orig & -> & -> & % & % & % & % & % & HGs & HLs)".
+    iMod "Hmask" as "_".
+    iMod ("Hclose" with "[HGs Hstate Htok]") as "_".
+    { iNext.
+      iDestruct "Hstate" as "[->|[Hstate|[Hstate|Hstate]]]".
+      - iExists {[add_1_ev]}.
+        rewrite left_id_L.
+        iFrame "HGs"; eauto.
+      - iDestruct "Hstate" as (?) "[? Htok']".
+        iDestruct (own_valid_2 with "Htok Htok'") as %?; done.
+      - iDestruct "Hstate" as (?) "[(%&%&%) Htok']"; simplify_eq.
+        iExists _; iFrame "HGs".
+        iRight; iRight; iRight.
+        iExists add_1_ev, ev; iFrame.
+        iPureIntro.
+        split_and!; [set_solver|done|done|done|done].
+      - iDestruct "Hstate" as (? ?) "(? & Htok' & ?)".
+        iDestruct (own_valid_2 with "Htok Htok'") as %?; done. }
+    iModIntro.
+    wp_pures.
+    wp_apply "Hget"; first done.
+    iMod fupd_mask_subseteq as "Hmask"; [|iModIntro]; [solve_ndisj|].
+    iExists _, _; iFrame "HLs".
+    iNext.
+    iIntros (s3 pst lst) "(% & HLs & %Hop & %Hst)".
+    iMod "Hmask" as "_".
+    iInv use_case_inv_name as (ges') ">[HGs Hstate]" "Hclose".
+    iDestruct (LocState_TakeSnap with "HLs") as "[HLs HLsnap]".
+    assert (↑CRDT_InvName ⊆ ⊤ ∖ ↑use_case_inv_name) by solve_ndisj.
+    iMod (GlobState_TakeSnap with "[//] HGs") as "[HGs HGsnap]"; first done.
+    iMod (LocSnap_GlobSnap_Provenance' with "[//] HGsnap HLsnap") as (h) "(#HGsnap & % & %)";
+      first done.
+    iMod (GlobSnap_GlobState_Included with "[//] HGsnap HGs") as "[% HGs]"; first done.
+    assert (h = ges') as -> by set_solver.
+    iDestruct "Hstate" as "[->|[Hstate|[Hstate|Hstate]]]".
+    - set_solver.
+    - iDestruct "Hstate" as (ev) "[(%&%Hev_val&%) Htk]"; simplify_eq.
+      assert (add_1_ev = ev) as <- by set_solver.
+      assert ({[add_1_ev]} ∪ s3 = {[add_1_ev]}) as Hunion_eq by set_solver.
+      rewrite Hunion_eq in Hst.
+      rewrite /crdt_denot /= /ctr_denot elements_singleton /= /ctr_payload Hev_val in Hst; subst.
+      rewrite /StLib_St_Coh /= /Ctr_St_Coh in Hop; subst.
+      iMod ("Hclose" with "[HGs Htk]") as "_".
+      { iNext. iExists _; iFrame "HGs"; eauto. }
+      iModIntro.
+      do 2 wp_pure _.
+      wp_apply assert_proof.wp_assert.
+      wp_pures. iSplit; first done.
+      iNext; iApply "HΦ"; done.
+    - iDestruct "Hstate" as (ev) "[(%&%Hev_val&%) Htk]"; simplify_eq.
+      assert (add_1_ev = ev) as <- by set_solver.
+      iDestruct (LocState_OwnOrig with "HLs") as %Horigs.
+      assert (EV_Orig add_1_ev = 0%nat); last congruence.
+      apply Horigs; set_solver.
+    - iDestruct "Hstate" as (ev1 ev2) "[(%&%Hev1_val&%&%Hev2_val&%) [Htk1 Htk2]]"; simplify_eq.
+      iDestruct (LocState_OwnOrig with "HLs") as %Horigs.
+      assert (EV_Orig add_1_ev = 0%nat).
+      { apply Horigs; set_solver. }
+      assert (add_1_ev = ev1 ∨ add_1_ev = ev2) as [|] by set_solver; [subst|congruence].
+      assert ({[ev1]} ∪ s3 = {[ev1]} ∨ {[ev1]} ∪ s3 = {[ev1; ev2]}) as Hunion_eq.
+      { destruct (decide (ev2 ∈ s3)).
+        - right; set_solver.
+        - left; set_solver. }
+      destruct Hunion_eq as [Hunion_eq|Hunion_eq].
+      + rewrite Hunion_eq in Hst.
+        rewrite /crdt_denot /= /ctr_denot elements_singleton /= /ctr_payload Hev1_val in Hst; subst.
+        rewrite /StLib_St_Coh /= /Ctr_St_Coh in Hop; subst.
+        iMod ("Hclose" with "[HGs Htk1 Htk2]") as "_".
+        { iNext. iExists _; iFrame "HGs"; iRight; iRight; iRight; iExists _, _; iFrame; eauto. }
+        iModIntro.
+        do 2 wp_pure _.
+        wp_apply assert_proof.wp_assert.
+        wp_pures. iSplit; first done.
+        iNext; iApply "HΦ"; done.
+      + assert (ev1 ≠ ev2) by congruence.
+        rewrite Hunion_eq in Hst.
+        rewrite /crdt_denot /= /ctr_denot in Hst.
+        erewrite ctr_value_perm in Hst; last by apply elements_disj_union; set_solver.
+        rewrite !elements_singleton /= /ctr_payload Hev1_val Hev2_val in Hst.
+        rewrite /StLib_St_Coh /= /Ctr_St_Coh in Hop; subst.
+        iMod ("Hclose" with "[HGs Htk1 Htk2]") as "_".
+        { iNext. iExists _; iFrame "HGs"; iRight; iRight; iRight; iExists _, _; iFrame; eauto. }
+        iModIntro.
+        do 2 wp_pure _.
+        wp_apply assert_proof.wp_assert.
+        wp_pures. iSplit; first done.
+        iNext; iApply "HΦ"; done.
+  Qed.
+
+  Program Definition Ifin : fin (length addresses).
+  Proof. apply (@Fin.of_nat_lt 1 (length addresses)); simpl; lia. Defined.
+
+  Lemma wp_use_case_program2 `{!StLib_Res CtrOp} γ1 γ2 :
+    {{{ GlobInv ∗ StLib_InitToken Ifin ∗ pn_init_crdt_spec pncounter_init ∗
+        ([∗ list] i↦z ∈ CRDT_Addresses, z ⤇ StLib_SocketProto) ∗
+        SocketAddressInet "1.1.1.2" 100 ⤳ (∅, ∅) ∗ free_ports "1.1.1.2" {[100%positive]} ∗
+        inv use_case_inv_name (use_case_inv γ1 γ2) ∗ own γ2 (Excl ()) }}}
+      use_case_program2 @["1.1.1.2"]
+    {{{ RET #(); True }}}.
+  Proof.
+    iIntros (Φ)
+      "(#HGinv & Hcrdt_tk & Hinit& #Hprotos & Hsa & Hfp & #Hinv & Htok) HΦ".
+    rewrite /use_case_program2.
+    wp_apply ("Hinit" $! _ (SocketAddressInet "1.1.1.2" 100) addresses_val
+               with "[$Hsa $Hfp $Hcrdt_tk]").
+    { iFrame "#".
+      iSplit; first by iPureIntro; apply is_list_inject.
+      iPureIntro; set_solver. }
+    iIntros (get upd) "(Hls & #Hget & #Hupd)".
+    wp_pures.
+    wp_apply ("Hupd" $! _ (Add _)); [done|done|].
+    iInv use_case_inv_name as (ges) ">[HGs Hstate]" "Hclose".
+    iMod fupd_mask_subseteq as "Hmask"; [|iModIntro]; [solve_ndisj|].
+    iExists _, _, _; iFrame.
+    iNext.
+    iIntros (add_2_ev h' s1' s2').
+    rewrite !left_id_L.
+    iIntros "(%Hadd_2_val & %Hadd_2_orig & -> & -> & % & % & % & % & % & HGs & HLs)".
+    iMod "Hmask" as "_".
+    iMod ("Hclose" with "[HGs Hstate Htok]") as "_".
+    { iNext.
+      iDestruct "Hstate" as "[->|[Hstate|[Hstate|Hstate]]]".
+      - iExists {[add_2_ev]}.
+        rewrite left_id_L.
+        iFrame "HGs"; eauto 10.
+      - iDestruct "Hstate" as (?) "[(%&%&%) Htok']"; simplify_eq.
+        iExists _; iFrame "HGs".
+        iRight; iRight; iRight.
+        iExists ev, add_2_ev; iFrame.
+        iPureIntro.
+        split_and!; [set_solver|done|done|done|done].
+      - iDestruct "Hstate" as (?) "[? Htok']".
+        iDestruct (own_valid_2 with "Htok Htok'") as %?; done.
+      - iDestruct "Hstate" as (? ?) "(? & ? & Htok')".
+        iDestruct (own_valid_2 with "Htok Htok'") as %?; done. }
+    iModIntro.
+    wp_pures.
+    wp_apply "Hget"; first done.
+    iMod fupd_mask_subseteq as "Hmask"; [|iModIntro]; [solve_ndisj|].
+    iExists _, _; iFrame "HLs".
+    iNext.
+    iIntros (s3 pst lst) "(% & HLs & %Hop & %Hst)".
+    iMod "Hmask" as "_".
+    iInv use_case_inv_name as (ges') ">[HGs Hstate]" "Hclose".
+    iDestruct (LocState_TakeSnap with "HLs") as "[HLs HLsnap]".
+    assert (↑CRDT_InvName ⊆ ⊤ ∖ ↑use_case_inv_name) by solve_ndisj.
+    iMod (GlobState_TakeSnap with "[//] HGs") as "[HGs HGsnap]"; first done.
+    iMod (LocSnap_GlobSnap_Provenance' with "[//] HGsnap HLsnap") as (h) "(#HGsnap & % & %)";
+      first done.
+    iMod (GlobSnap_GlobState_Included with "[//] HGsnap HGs") as "[% HGs]"; first done.
+    assert (h = ges') as -> by set_solver.
+    iDestruct "Hstate" as "[->|[Hstate|[Hstate|Hstate]]]".
+    - set_solver.
+    - iDestruct "Hstate" as (ev) "[(%&%Hev_val&%) Htk]"; simplify_eq.
+      assert (add_2_ev = ev) as <- by set_solver.
+      iDestruct (LocState_OwnOrig with "HLs") as %Horigs.
+      assert (EV_Orig add_2_ev = 1%nat); last congruence.
+      apply Horigs; set_solver.
+    - iDestruct "Hstate" as (ev) "[(%&%Hev_val&%) Htk]"; simplify_eq.
+      assert (add_2_ev = ev) as <- by set_solver.
+      assert ({[add_2_ev]} ∪ s3 = {[add_2_ev]}) as Hunion_eq by set_solver.
+      rewrite Hunion_eq in Hst.
+      rewrite /crdt_denot /= /ctr_denot elements_singleton /= /ctr_payload Hev_val in Hst; subst.
+      rewrite /StLib_St_Coh /= /Ctr_St_Coh in Hop; subst.
+      iMod ("Hclose" with "[HGs Htk]") as "_".
+      { iNext. iExists _; iFrame "HGs"; eauto 10. }
+      iModIntro.
+      do 2 wp_pure _.
+      wp_apply assert_proof.wp_assert.
+      wp_pures. iSplit; first done.
+      iNext; iApply "HΦ"; done.
+    - iDestruct "Hstate" as (ev1 ev2) "[(%&%Hev1_val&%&%Hev2_val&%) [Htk1 Htk2]]"; simplify_eq.
+      iDestruct (LocState_OwnOrig with "HLs") as %Horigs.
+      assert (EV_Orig add_2_ev = 1%nat).
+      { apply Horigs; set_solver. }
+      assert (add_2_ev = ev1 ∨ add_2_ev = ev2) as [|] by set_solver; [congruence|subst].
+      assert ({[ev2]} ∪ s3 = {[ev2]} ∨ {[ev2]} ∪ s3 = {[ev1; ev2]}) as Hunion_eq.
+      { destruct (decide (ev1 ∈ s3)).
+        - right; set_solver.
+        - left; set_solver. }
+      destruct Hunion_eq as [Hunion_eq|Hunion_eq].
+      + rewrite Hunion_eq in Hst.
+        rewrite /crdt_denot /= /ctr_denot elements_singleton /= /ctr_payload Hev2_val in Hst; subst.
+        rewrite /StLib_St_Coh /= /Ctr_St_Coh in Hop; subst.
+        iMod ("Hclose" with "[HGs Htk1 Htk2]") as "_".
+        { iNext. iExists _; iFrame "HGs"; iRight; iRight; iRight; iExists _, _; iFrame; eauto. }
+        iModIntro.
+        do 2 wp_pure _.
+        wp_apply assert_proof.wp_assert.
+        wp_pures. iSplit; first done.
+        iNext; iApply "HΦ"; done.
+      + assert (ev1 ≠ ev2) by congruence.
+        rewrite Hunion_eq in Hst.
+        rewrite /crdt_denot /= /ctr_denot in Hst.
+        erewrite ctr_value_perm in Hst; last by apply elements_disj_union; set_solver.
+        rewrite !elements_singleton /= /ctr_payload Hev1_val Hev2_val in Hst.
+        rewrite /StLib_St_Coh /= /Ctr_St_Coh in Hop; subst.
+        iMod ("Hclose" with "[HGs Htk1 Htk2]") as "_".
+        { iNext. iExists _; iFrame "HGs"; iRight; iRight; iRight; iExists _, _; iFrame; eauto. }
+        iModIntro.
+        do 2 wp_pure _.
+        wp_apply assert_proof.wp_assert.
+        wp_pures. iSplit; first done.
+        iNext; iApply "HΦ"; done.
+  Qed.
+
+End use_case_proof.
+
+Section program_proof.
+  Context `{!anerisG M Σ} `{!inG Σ (exclR unitO)}.
+  Context `{!@StLibG CtrOp _ _ Σ}.
+
+  Global Instance pn_cpt_init_cl : StLib_Init_Function := {| init := pn_cpt_init |}.
+
+  Lemma wp_use_case_program :
+    ⊢ |={⊤}=> ∃ Res : StLib_Res (prodOp gctr_op gctr_op),
+         ([∗ list] i↦z ∈ CRDT_Addresses, z ⤇ StLib_SocketProto) -∗
+         free_ip "1.1.1.1" -∗
+         free_ip "1.1.1.2" -∗
+         SocketAddressInet "1.1.1.1" 100 ⤳ (∅, ∅) -∗
+         SocketAddressInet "1.1.1.2" 100 ⤳ (∅, ∅) -∗
+         WP use_case_program @["system"]
+      {{ v, ⌜v = #()⌝ }}.
+  Proof.
+    iIntros "".
+    iMod (@StLibSetup_Init
+            (prodOp gctr_op gctr_op) (prodSt gctr_st gctr_st)
+            _ _ _ _ _ _ (prod_lattice (vectn_le_lat _) (vectn_le_lat _))
+            (prod_params gctr_op gctr_st gctr_op gctr_st) pn_cpt_init_cl with "[//]")
+      as (Res) "(#HGinv & HGs & Htks & #Hinit)".
+    admit.
+    iExists Res.
+    iModIntro.
+    iIntros "#Hprotos Hfip1 Hfip2 Hsa1 Hsa2".
+    admit.
+  Admitted.
+  (*  iDestruct "Htks" as "(Hitk1 & Hitk2 & _)".
+    rewrite /use_case_program.
+    iMod (own_alloc (Excl ())) as (γ1) "Htk1"; first done.
+    iMod (own_alloc (Excl ())) as (γ2) "Htk2"; first done.
+    iMod (inv_alloc use_case_inv_name _ (use_case_inv γ1 γ2) with "[HGs]") as "#Hinv".
+    { iNext; iExists _; iFrame. iLeft; done. }
+    wp_apply aneris_wp_start; first done.
+    iSplitL "Hfip1"; first by iNext.
+    iSplitR "Hitk1 Hsa1 Htk1"; last first.
+    { iNext. iIntros "Hfps".
+      iApply (wp_use_case_program1 with "[$]"); done. }
+    iNext.
+    wp_pures.
+    wp_apply aneris_wp_start; first done.
+    iSplitL "Hfip2"; first by iNext.
+    iSplit; first done.
+    iNext. iIntros "Hfps".
+    iApply (wp_use_case_program2 with "[$]"); done.
+  Qed.
+
+End use_case_proof. *)
+End program_proof.
+(*
+Definition init_state :=
+  {|
+    state_heaps := {[ "system" := ∅ ]};
+    state_sockets := {[ "system" := ∅ ]};
+    state_ports_in_use := {["1.1.1.1" := ∅; "1.1.1.2" := ∅ ]};
+    state_ms := ∅;
+  |}.
+
+Definition Trivial_Mdl : resources.Model :=
+  {| model_state := ();
+    model_rel := λ _ _, True;
+    model_state_initial := (); |}.
+
+Lemma Trivial_Mdl_finitary : aneris_model_rel_finitary Trivial_Mdl.
+Proof. intros ?. apply finite_smaller_card_nat. apply _. Qed.
+
+
+Definition use_case_Σ := #[anerisΣ Trivial_Mdl; RCBΣ; @OPLIBΣ CtrOp _ _; GFunctor (exclR unitO)].
+
+Theorem use_case_program_adequate :
+  aneris_adequate use_case_program "system" init_state (λ v, v = #()).
+Proof.
+  eapply (@adequacy
+            use_case_Σ Trivial_Mdl _ _ {["1.1.1.1"; "1.1.1.2"]}
+            (list_to_set addresses) ∅ ∅ ∅);
+    [apply Trivial_Mdl_finitary| |set_solver..|done|done].
+  iIntros (HanerisG) "".
+  iModIntro.
+  iIntros "Hfx Hsas _ Hfips _ _ _ _ _".
+  rewrite big_sepS_union; last set_solver.
+  rewrite !big_sepS_singleton.
+  unfold addresses.
+  iDestruct "Hfips" as "[Hfip1 Hfip2]".
+  iAssert (SocketAddressInet "1.1.1.1" 100 ⤳ (∅, ∅) ∗
+           SocketAddressInet "1.1.1.2" 100 ⤳ (∅, ∅))%I with "[Hsas]" as "[Hsa1 Hsa2]".
+  { rewrite !list_to_set_cons list_to_set_nil right_id_L.
+    rewrite big_sepS_union; last set_solver.
+    rewrite !big_sepS_singleton.
+    repeat (rewrite bool_decide_eq_false_2; last set_solver).
+    done. }
+  iMod wp_use_case_program as (Res) "Hwp".
+  iD  estruct (unallocated_split with "Hfx") as "[Hfx0 Hfx]"; [set_solver|].
+  iDestruct (unallocated_split with "Hfx") as "[Hfx1 _]"; [set_solver|].
+  iApply (aneris_wp_socket_interp_alloc_singleton
+            (@OpLib_SocketProto _ _ _ _ _ _ _ Res 0) with "Hfx0").
+  iIntros "#Hsi0".
+  iApply (aneris_wp_socket_interp_alloc_singleton
+            (@OpLib_SocketProto _ _ _ _ _ _ _ Res 1) with "Hfx1").
+  iIntros "#Hsi1".
+  iAssert ([∗ list] i↦z ∈ addresses, z ⤇ (@OpLib_SocketProto _ _ _ _ _ _ _ Res i))%I as "Hprotos".
+  { repeat iSplit; done. }
+  wp_apply ("Hwp" with "Hprotos Hfip1 Hfip2 Hsa1 Hsa2").
+Qed.
+
+*)
+
+
+
+(* Section OpPNCounter. *)
+
+(*   Context `{!Log_Time}. *)
+
+(*   Definition op_ctr_effect st (ev : Event CtrOp) st' := *)
+(*     st' = (st + ctr_payload ev.(EV_Op))%Z. *)
+
+(*   Lemma op_ctr_effect_fun st : Rel2__Fun (op_ctr_effect st). *)
+(*   Proof. *)
+(*     constructor. unfold op_ctr_effect. *)
+(*     intros a b b' Hb Hb'. *)
+(*     destruct (EV_Op a) as [z]; simpl in *; subst; auto. *)
+(*   Qed. *)
+
+
+(*   Lemma ctr_denot_union (s : gset (Event CtrOp)) (ev : Event CtrOp) (res : CtrSt) : *)
+(*     ⟦ s ⟧ ⇝ res -> *)
+(*     ev ∉ s -> *)
+(*     ⟦ s ∪ {[ ev ]} ⟧ ⇝ (res + ctr_payload ev.(EV_Op))%Z. *)
+(*   Proof. *)
+(*     simpl. unfold ctr_denot. *)
+(*     intros -> Hnotin. *)
+(*     assert (s ## {[ ev ]}) as Hdisj by set_solver. *)
+(*     pose proof (elements_disj_union s *)
+(*                                     ({[ev]} : gset (Event CtrOp)) *)
+(*                                     Hdisj) as Hperm. *)
+(*     apply ctr_value_perm in Hperm. rewrite Hperm. *)
+(*     by rewrite elements_singleton ctr_value_app ctr_value_singleton. *)
+(*   Qed. *)
+
+(*    Definition op_ctr_init_st := 0%Z. *)
+
+(*   Lemma op_ctr_init_st_coh : ⟦ (∅ : gset (Event CtrOp)) ⟧ ⇝ op_ctr_init_st. *)
+(*   Proof. done. Qed. *)
+
+(*  End OpPNCounter. *)
+
+
+(* Notation pnParams := (prod_params gctr_op gctr_st gctr_op gctr_st). *)
+
+  (* Definition init_val_pn : val := *)
+  (*   (statelib_init *)
+  (*        (prod_ser *)
+  (*           (gctr_params.(StLib_CohParams).(StLib_StSerialization).(s_serializer)).(s_ser) *)
+  (*           (gctr_params.(StLib_CohParams).(StLib_StSerialization).(s_serializer)).(s_ser)) *)
+  (*        (prod_deser *)
+  (*           (gctr_params.(StLib_CohParams).(StLib_StSerialization).(s_serializer)).(s_deser) *)
+  (*           (gctr_params.(StLib_CohParams).(StLib_StSerialization).(s_serializer)).(s_deser))). *)
+
+  (* Definition init_spec_pn  := *)
+  (* @init_spec *)
+  (*     _ _ _ _ _ _ _ _ _ pnParams stparams0 init_val_pn. *)
